Kami/Syntax.v
@@ -678,9 +678,10 @@ Definition Void := Bit 0.
 
 Record PrimitiveModule :=
   { pm_name: string;
-    (* [pm_args] is not used in Kami at all;
+    (* [pm_args] and [pm_consts] are not used in Kami at all;
      * it's just to provide information to the pretty-printer. *)
     pm_args: list (Attribute Kind);
+    pm_consts: list (Attribute {k: Kind & ConstT k});
     pm_regInits: list RegInitT;
     pm_rules: list (Attribute (Action Void));
     pm_methods: list DefMethT }.
